Generalizing some of the lemmas to avoid duplicating too much effort.

theories/newth/NewFMap.ec
@@ -3,108 +3,78 @@
  * Distributed under the terms of the CeCILL-C license
  * -------------------------------------------------------------------- *)
 
-require import Pred.
-require import Option.
-require import Pair.
-require import Int.
-require import NewList.
-require import NewFSet.
+require import Fun Pred Option Pair Int NewList NewFSet.
 
+pragma +implicits.
+
+(*
 op reduce (xs : ('a * 'b) list) : ('a * 'b) list =
   foldl (fun aout (kv : 'a * 'b) =>
     if mem [] kv.`1 then aout else kv :: aout)
-  [] xs.
+  [] xs. *)
+
+(** Even more general (to NewList?) **)
+lemma uniq_map_uniq (xs : 'a list) (f : 'a -> 'c):
+  uniq (map f xs) => uniq xs.
+proof.
+  elim xs=> //= x xs IH [] x1_notin_fxs /IH -> /=.
+  rewrite -not_def=> x_in_xs; move: x1_notin_fxs=> //=. (* This is a weird way of contraposing *)
+  by rewrite -has_pred1 has_map hasP; exists x.
+qed.
+
+lemma perm_eq_uniq_map (f : 'a -> 'b)  (s1 s2 : 'a list):
+  perm_eq s1 s2 => uniq (map f s1) <=> uniq (map f s2).
+proof. by move=> /(perm_eq_map f) /perm_eq_uniq ->. qed.
 
 (* TODO: this may be of more general interest and may benefit from a
          move to NewList, or a separate PairList theory. *)
-op fst (xs : ('a * 'b) list) =
-  with xs = "[]"      => []
-  with xs = (::) x xs => x.`1::fst xs.
-
-op snd (xs : ('a * 'b) list) =
-  with xs = "[]"      => []
-  with xs = (::) x xs => x.`2::snd xs.
-
 op undup_fst (xs : ('a * 'b) list) =
   with xs = "[]"      => []
-  with xs = (::) x xs => if mem (fst xs) x.`1
+  with xs = (::) x xs => if mem (map fst xs) x.`1
                          then undup_fst xs
                          else x::undup_fst xs.
 
-op uniq_fst (xs : ('a * 'b) list) =
-  with xs = "[]"      => true
-  with xs = (::) x xs => !mem (fst xs) x.`1 /\ uniq_fst xs.
-
-lemma mem_fst_mem (xs : ('a * 'b) list) (ab : 'a * 'b):
-  mem xs ab => mem (fst xs) ab.`1.
-proof.
-  by elim xs=> //= x xs IH [-> //= | /IH ->].
-qed.
-
-lemma mem_snd_mem (xs : ('a * 'b) list) (ab : 'a * 'b):
-  mem xs ab => mem (snd xs) ab.`2.
-proof.
-  by elim xs=> //= x xs IH [-> //= | /IH ->].
-qed.
-
 lemma mem_fst_ex_snd (xs : ('a * 'b) list) (x : 'a):
-  mem (fst xs) x <=> (exists y, mem xs (x,y)).
+  mem (map fst xs) x <=> (exists y, mem xs (x,y)).
 proof.
-  split; last by move=> [] y /mem_fst_mem.
-  elim xs=> //= [[a b]] xs IH /= [].
-    by move=> -> /=; exists b.
-  by move=> /IH [] y xy_in_xs; exists y; right.
+  rewrite -has_pred1 has_map hasP /preim/fst/pred1; split.
+    by move=> [[a b]] [x0_in_xs ->>]; exists b.
+  by move=> [y] xs_in_xs; exists (x,y).
 qed.
 
 lemma mem_snd_ex_fst (xs : ('a * 'b) list) (y : 'b):
-  mem (snd xs) y <=> (exists x, mem xs (x,y)).
+  mem (map snd xs) y <=> (exists x, mem xs (x,y)).
 proof.
-  split; last by move=> [] x /mem_snd_mem.
-  elim xs=> //= [[a b]] xs IH /= [].
-    by move=> -> /=; exists a.
-  by move=> /IH [] x xy_in_xs; exists x; right.
-qed.
-
-lemma uniq_fst_uniq_fst (xs : ('a * 'b) list):
-  uniq_fst xs =>
-  uniq (fst xs).
-proof.
-  by elim xs=> //= x xs IH [] ->.
-qed.
-
-lemma uniq_fst_uniq (xs : ('a * 'b) list):
-  uniq_fst xs =>
-  uniq xs.
-proof.
-  elim xs=> //= x xs IH [] x1_notin_fstxs /IH uniq_xs.
-  by split=> //; rewrite -not_def=> /mem_fst_mem.
+  rewrite -has_pred1 has_map hasP /preim/fst/pred1; split.
+    by move=> [[a b]] [x0_in_xs ->>]; exists a.
+  by move=> [x] xs_in_xs; exists (x,y).
 qed.
 
 lemma mem_fst_undup_fst (xs : ('a * 'b) list):
-  mem (fst (undup_fst xs)) <= mem (fst xs).
+  mem (map fst (undup_fst xs)) <= mem (map fst xs).
 proof.
   elim xs=> //= x xs IH.
-  case (mem (fst xs) x.`1).
+  case (mem (map fst xs) x.`1).
     by move=> x1_in_fstxs a /IH; rewrite in_cons=> ->.
     by move=> x1_notin_fstxs a; rewrite !in_cons=> [-> | /IH ->].
 qed.
 
-lemma uniq_undup_fst (xs : ('a * 'b) list): uniq_fst (undup_fst xs).
+lemma uniq_undup_fst (xs : ('a * 'b) list): uniq (map fst (undup_fst xs)).
 proof.
   elim xs=> //= x xs IH.
-  case (mem (fst xs) x.`1)=> //=.
-  rewrite IH /= => x1_notin_fstundup; rewrite -not_def.
-  by move=> /mem_fst_undup_fst.
+  case (mem (map fst xs) x.`1)=> //=.
+  rewrite IH /= => x1_notin_fstundup.
+  by rewrite -not_def=> /mem_fst_undup_fst.
 qed.
 
-lemma uniq_perm_eq_fst (s1 s2 : ('a * 'b) list):
-  uniq_fst s1 =>
-  uniq_fst s2 =>
+lemma uniq_perm_eq_map (s1 s2 : ('a * 'b) list) (f: 'a * 'b -> 'c):
+  uniq (map f s1) =>
+  uniq (map f s2) =>
   (forall (x : 'a * 'b), mem s1 x <=> mem s2 x) =>
   perm_eq s1 s2.
 proof.
   move=> Us1 Us2 eq12; rewrite /perm_eq allP => x _ /=.
-  by rewrite !count_uniq_mem 3:eq12 //; apply uniq_fst_uniq.
+  by rewrite !count_uniq_mem 3:eq12 //; apply @(uniq_map_uniq _ f).
 qed.
 
 (* -------------------------------------------------------------------- *)
@@ -119,10 +89,12 @@ op oflist : ('a * 'b) list -> ('a,'b) fmap.
 axiom elemsK  (m : ('a,'b) fmap): Self.oflist (elems  m) = m.
 axiom oflistK (s : ('a * 'b) list): perm_eq (undup_fst s) (elems (Self.oflist s)).
 
-lemma uniq_keys (m : ('a,'b) fmap): uniq_fst (elems m).
+lemma uniq_keys (m : ('a,'b) fmap): uniq (map fst (elems m)).
 proof.
-  rewrite -(elemsK m); move: (elems m) => {m} m.
-  admit. (* TODO: fill in this proof *)
+  rewrite -elemsK; move: (elems m) => {m} m.
+  apply @(perm_eq_uniq (map fst (undup_fst m)) _).
+    by apply perm_eq_map; apply oflistK.
+  by apply uniq_undup_fst.
 qed.
 
 axiom fmap_eq (s1 s2 : ('a,'b) fmap):
@@ -141,23 +113,24 @@ op get (xs : ('a * 'b) list) (a : 'a) =
                          else get xs a.
 
 lemma mem_get_uniq (xs : ('a * 'b) list) (a : 'a) (b : 'b):
-  uniq_fst xs =>
+  uniq (map fst xs) =>
   mem xs (a,b) <=> get xs a = Some b.
 proof.
+  (** This feels larger than necessary **)
   elim xs=> //= [[a' b']] xs IH /= [].
   move=> a'_notin_fstxs uniq_xs; split.
     case=> [[-> ->] // | H].
-    cut:= H => /mem_fst_mem; case (a = a')=> //= _ _.
-    by rewrite -IH.
+    cut: mem (map fst xs) a
+      by rewrite -has_pred1 has_map hasP; exists (a,b).
+    move: a'_notin_fstxs; rewrite {2}/fst //=.
+    by case (a = a')=> //= [-> -> // | _ _ _]; rewrite -IH.
   case (a = a')=> //= [_ /someI // | ].
   by rewrite -IH.
 qed.
 
 lemma get_mem (xs : ('a * 'b) list) (x : 'a):
   get xs x <> None <=> mem xs (x,oget (get xs x)).
-proof.
-  by elim xs=> //= [[a b]] xs IH /=; case (x = a).
-qed.
+proof. by elim xs=> //= [[a b]] xs IH /=; case (x = a). qed.
 
 op "_.[_]" (m : ('a,'b) fmap) (x : 'a) = get (elems m) x
   axiomatized by getE.
@@ -165,14 +138,25 @@ op "_.[_]" (m : ('a,'b) fmap) (x : 'a) = get (elems m) x
 lemma mapP (m1 m2 : ('a,'b) fmap):
   (m1 = m2) <=> (forall x, m1.[x] = m2.[x]).
 proof.
-  split=> [-> // | H]; apply fmap_eq; apply uniq_perm_eq;
-    first 2 by apply uniq_fst_uniq; apply uniq_keys.
+  split=> // H; apply fmap_eq; apply uniq_perm_eq;
+    first 2 by apply @(uniq_map_uniq _ fst); apply uniq_keys.
   move: H; rewrite getE /= => H [a b].
   by rewrite !mem_get_uniq 1..2:uniq_keys // H.
 qed.
 
 (* -------------------------------------------------------------------- *)
-op dom (m : ('a,'b) fmap) = NewFSet.oflist (fst (elems m))
+op set (xs : ('a * 'b) list) (a : 'a) (b : 'b) =
+  with xs = "[]"      => [(a,b)]
+  with xs = (::) x xs => if a = x.`1
+                         then (a,b)::xs
+                         else x::(set xs a b).
+
+op "_.[_<-_]" (m : ('a,'b) fmap) (a : 'a) (b : 'b) =
+  Self.oflist (set (elems m) a b)
+axiomatized by setE.
+
+(* -------------------------------------------------------------------- *)
+op dom (m : ('a,'b) fmap) = NewFSet.oflist (map fst (elems m))
   axiomatized by domE.
 
 lemma in_dom (m: ('a,'b) fmap) (a : 'a):
@@ -182,11 +166,11 @@ proof.
   split.
     rewrite mem_fst_ex_snd=> [] b.
     by rewrite mem_get_uniq 1:uniq_keys // => ->.
-  by rewrite get_mem=> /mem_fst_mem.
+  by rewrite get_mem=> H; rewrite -has_pred1 has_map hasP; exists (a,oget (get (elems m) a)).
 qed.
 
 (* -------------------------------------------------------------------- *)
-op rng (m : ('a,'b) fmap) = NewFSet.oflist (snd (elems m))
+op rng (m : ('a,'b) fmap) = NewFSet.oflist (map snd (elems m))
   axiomatized by rngE.
 
 lemma in_rng (m: ('a,'b) fmap) (b : 'b):
@@ -196,7 +180,7 @@ proof.
   split.
     rewrite mem_snd_ex_fst=> [] a.
     by rewrite mem_get_uniq 1:uniq_keys // => a_in_m; exists a.
-  by move=> [] a; rewrite -mem_get_uniq 1:uniq_keys // => /mem_snd_mem.
+  by move=> [] a; rewrite -mem_get_uniq 1:uniq_keys // => H; rewrite -has_pred1 has_map hasP; exists (a,b).
 qed.
 
 (* -------------------------------------------------------------------- *)
